src/DxInstructions.v
@@ -518,17 +518,19 @@ Fixpoint bpf_interpreter_aux (fuel: nat) {struct fuel}: M unit :=
   | S fuel0 =>
     do len  <-- eval_ins_len;
     do pc   <-- eval_pc;
-      if (Int_leu int32_0 pc) then
-        if (Int.ltu pc len) then (**r 0 < pc < len: pc is less than the length of l *)
-          do _ <-- step;
-          do f <-- eval_flag;
-            if flag_eq f BPF_OK then
-              do _ <-- upd_pc_incr;
-                bpf_interpreter_aux fuel0
-            else
-              returnM tt
-        else
-          upd_flag BPF_ILLEGAL_LEN
+      if (Int.ltu pc len) then (**r 0 < pc < len: pc is less than the length of l *)
+        do _ <-- step;
+        do f <-- eval_flag;
+          if flag_eq f BPF_OK then
+            do len0  <-- eval_ins_len;
+            do pc0   <-- eval_pc;
+              if (Int.ltu (Int.add pc0 int32_1) len0) then
+                do _ <-- upd_pc_incr;
+                  bpf_interpreter_aux fuel0
+              else
+                upd_flag BPF_ILLEGAL_LEN
+          else
+            returnM tt
       else
         upd_flag BPF_ILLEGAL_LEN
   end.
