isolation/VerifierInv.v
@@ -1,0 +1,185 @@
+From compcert Require Import Integers Values.
+From bpf.comm Require Import Regs State LemmaNat.
+From bpf.model Require Import Semantics.
+From bpf.isolation Require Import AlignChunk CommonISOLib.
+From Coq Require Import ZArith Lia List.
+Import ListNotations.
+
+Open Scope Z_scope.
+
+Ltac destruct_if_zeqb Hname :=
+  match goal with
+  | |- context [(if ?X then _ else _) = Some _] =>
+    destruct X eqn: Hname;
+    [ eexists; rewrite Z.eqb_eq in Hname; rewrite Hname;
+  reflexivity |
+      rewrite Z.eqb_neq in Hname]
+  end.
+
+(**r CertrBPF needs the following two properties guaranteed by an assumed rbpf verifier, we will implement a verified verifier later~
+
+\begin{enumerate}
+    \item dst \& src registers are in [0, 10].
+    \item all jump operations are always within in bound.
+    tbc...
+    \item when ins.opcode = div, ins.src != 0
+    \item when ins.opcode = shift (lsh/rsh/arsh), $0 \leq ins.src \leq 32/64$
+    \item etc... (more ambitious: {\color{red} check\_mem = true?}  ...)  
+\end{enumerate}
+
+ *)
+
+Definition well_dst (i: int64) : Prop :=
+  0 <= get_dst i <= 10.
+
+Definition well_src (i: int64) : Prop :=
+  0 <= get_src i <= 10.
+
+Definition well_list_range (l: list int64) : Prop :=
+  (**r (0, Int.max_unsigned/8): at least one instruction, and at most Int.max_unsigned/8 because of memory region *)
+  1 <= Z.of_nat (List.length l) /\
+  Z.of_nat (List.length l) * 8 <= Ptrofs.max_unsigned /\
+  (**r the last instruaction is always exit: to guarantee the next instruction of each instruction is within the bound *)
+  List.nth_error l (List.length l - 1) = Some (Int64.repr 0x95).
+
+(**r how to define valid instruction: according to its opcode? any other more efficient algorithms? *) (*
+Definition valid_instruction () *)
+
+Close Scope Z_scope.
+
+Open Scope nat_scope.
+
+Definition is_jump (i: int64) : bool :=
+  match get_opcode i with
+  | 0x05
+  | 0x15 | 0x1d
+  | 0x25 | 0x2d
+  | 0x35 | 0x3d
+  | 0xa5 | 0xad
+  | 0xb5 | 0xbd
+  | 0x45 | 0x4d
+  | 0x55 | 0x5d
+  | 0x65 | 0x6d
+  | 0x75 | 0x7d
+  | 0xc5 | 0xcd
+  | 0xd5 | 0xdd => true
+  | _    => false
+  end.
+
+Definition is_lddw (i: int64) : bool :=
+  match get_opcode i with
+  | 0x18 => true
+  | _    => false
+  end.
+
+Definition well_jump (i: int64) (pc len: nat) : Prop :=
+  if is_jump i then
+    let imm := Regs.get_offset i in
+    let pc'  :=Int.add (Int.repr (Z.of_nat pc)) imm in
+      Int.cmpu Clt pc' (Int.repr (Z.of_nat len)) = true
+  else
+    True.
+
+Definition well_lddw (i: int64) (pc len: nat) : Prop :=
+  if is_lddw i then
+    Int.cmpu Clt (Int.add (Int.repr (Z.of_nat pc)) Int.one) (Int.repr (Z.of_nat len)) = true
+  else
+    True.
+
+Definition verifier_inv' (l: list int64): Prop :=
+  well_list_range l /\
+  forall i, i < List.length l ->
+    match List.nth_error l i with
+    | Some ins =>
+        well_dst ins /\ well_src ins /\
+        well_lddw ins i (List.length l) /\
+        well_jump ins i (List.length l)
+    | None => False
+    end.
+
+Definition verifier_inv (st: state): Prop :=
+  (ins_len st) = (List.length (ins st))  /\
+  verifier_inv' (ins st).
+
+Close Scope nat_scope.
+
+Lemma verifier_inv_dst_reg:
+  forall ins,
+    well_dst ins ->
+    exists r,
+      Regs.int64_to_dst_reg' ins = Some r.
+Proof.
+  unfold well_dst, Regs.int64_to_dst_reg'; intros.
+  unfold z_to_reg.
+  remember (get_dst ins) as i.
+  clear Heqi.
+  destruct_if_zeqb Heq0.
+  destruct_if_zeqb Heq1.
+  destruct_if_zeqb Heq2.
+  destruct_if_zeqb Heq3.
+  destruct_if_zeqb Heq4.
+  destruct_if_zeqb Heq5.
+  destruct_if_zeqb Heq6.
+  destruct_if_zeqb Heq7.
+  destruct_if_zeqb Heq8.
+  destruct_if_zeqb Heq9.
+  destruct_if_zeqb Heq10.
+  lia.
+Qed.
+
+
+Lemma verifier_inv_src_reg :
+  forall ins,
+    well_src ins ->
+    exists r,
+      Regs.int64_to_src_reg' ins = Some r.
+Proof.
+  unfold well_src, Regs.int64_to_src_reg'; intros.
+  unfold z_to_reg.
+  remember (get_src ins) as i.
+  clear Heqi.
+  destruct_if_zeqb Heq0.
+  destruct_if_zeqb Heq1.
+  destruct_if_zeqb Heq2.
+  destruct_if_zeqb Heq3.
+  destruct_if_zeqb Heq4.
+  destruct_if_zeqb Heq5.
+  destruct_if_zeqb Heq6.
+  destruct_if_zeqb Heq7.
+  destruct_if_zeqb Heq8.
+  destruct_if_zeqb Heq9.
+  destruct_if_zeqb Heq10.
+  lia.
+Qed.
+
+Lemma opcode_and_255:
+  forall ins,
+    Nat.land (get_opcode ins) 255 = get_opcode ins.
+Proof.
+  intros.
+  unfold get_opcode.
+  unfold Int64.and.
+  change (Int64.unsigned (Int64.repr 255)) with (Z.of_nat (Z.to_nat 255)).
+  assert (Heq: Z.of_nat (Z.to_nat (Int64.unsigned ins)) = Int64.unsigned ins).
+  {
+    rewrite Z2Nat.id.
+    reflexivity.
+    apply Int64_unsigned_ge_0.
+  }
+  rewrite <- Heq; clear Heq.
+  rewrite land_land.
+  change (Z.to_nat 255) with 255%nat.
+  assert (Hrange: (Nat.land (Z.to_nat (Int64.unsigned ins)) 255 <= 255)%nat). {
+    rewrite Nat.land_comm.
+    rewrite land_bound.
+    lia.
+  }
+  assert (Hrange_z: (Z.of_nat (Nat.land (Z.to_nat (Int64.unsigned ins)) 255%nat) <= 255)%Z) by lia.
+  rewrite Int64.unsigned_repr.
+  rewrite Nat2Z.id.
+  rewrite <- Nat.land_assoc.
+  rewrite Nat.land_diag.
+  reflexivity.
+  change Int64.max_unsigned with 18446744073709551615%Z.
+  lia.
+Qed.
