equivalence/README.md
@@ -4,15 +4,13 @@ This folder is used to prove the equality among rbpf-coq interpreter (`model/`),
 
 *using the make command: `make equivalence`*
 
-**NB: The coq proof checking are time-costing because we must traverse `opcode \in [0,255]` in order to prove the different decoding ways are exactly same.**
-
 The two target thoerem are:
 
 ```Coq
 (**r equivalence1.v *)
 Theorem equivalence_between_formal_and_dx:
   forall f,
-    Semantics.bpf_interpreter f = DxInstructions.bpf_interpreter f.
+    Semantics.bpf_interpreter f = rBPFInterpreter.bpf_interpreter f.
     
 (**r equivalence2.v *)    
 Theorem equivalence_between_coq_and_dx_dx:
@@ -25,16 +23,7 @@ where `f` is a fuel to ensure that the coq functions always terminate.
 
 The equivalence proof between the later two models are simple: we only need to _unfold_ the renaming types/definitions of `DxInstructions.bpf_interpreter`, and simply _destruct_. So we mainly discuss the first equivalence proof idea:
 
-1. translating `model/Decode.get_instruction` (match-pattern version) to `switch.get_instruction_if` (if-then-else version), and proving that they are same
-
-```Coq
-(**r switch.v *)
-Lemma switch_if_same :
-  forall (opcode:nat) (rd rs:reg) (ofs: int) (i: int),
-    get_instruction opcode rd rs ofs i = get_instruction_if opcode rd rs ofs i.
-```
-
-2. proving each opcode of rbpf instructions are less or equal than 255 (because it only has 8-bits) so that if one opcode is greater than 255, we will get a contradiction in the hypothesis, then the rest proof is done!
+1. proving each opcode of rbpf instructions are less or equal than 255 (because it only has 8-bits) so that if one opcode is greater than 255, we will get a contradiction in the hypothesis, then the rest proof is done!
 
 ```Coq
 (**r equivalence.v *)
@@ -44,13 +33,10 @@ Lemma opcode_le_255 :
                   (Int64.and (State.eval_ins (State.eval_pc st) st) (Int64.repr 255))))%Z <= 255.
 ```
 
-3. considering the fact that the main difference between`Semantics.bpf_interpreter/Semantics.bpf_interpreter_aux` and `DxInstructions.bpf_interpreter/DxInstructions.bpf_interpreter_aux` is the `step` function, we prove the follow lemma.
+2. considering the fact that the main difference between`Semantics.bpf_interpreter/Semantics.bpf_interpreter_aux` and `rBPFInterpreter.bpf_interpreter/rBPFInterpreter.bpf_interpreter_aux` is the `step` function, we prove the follow lemma.
 ```Coq
 Lemma equivalence_between_formal_and_dx_step:
-  Semantics.step = DxInstructions.step.
+  Semantics.step = rBPFInterpreter.step.
 ```
 
-- we firstly discuss if opcode is one of the defined instructions, such `add64 dst imm (opcode = 0x07)`; 
-- then if we consider all defined instructions, we get the fact, `opcode <> 0x07/0x0f...`; 
-- the rest are all undefined instructions, so we traverse `opcode \in [0,255]`, and prove the other case in [0,255] are undefined;
-- finally, when `opcode > 255`, we use the lemma `opcode_le_255` to finish the whole proof.
+- we discuss each opcode
