isolation/README.md
@@ -1,7 +1,5 @@
 # Isolation proof (Certirbpf ensures the sandboxing property)
 
-*NB: The isolation proof only works on the commits before 2022-03-03, the ongoing modification will destroy the isolation proof. We plan to complete the simulation proof firstly and then add a new invariant called verifier_inv in order to prove the isolation property. The new invariant will be abandoned only when a verified rbpf verifier is done*
-
 This folder is used to prove the isolation property of the proof model (rbpf-coq interpreter).
 
 *using the make command: `make isolation`*
@@ -10,20 +8,22 @@ There are two target thoerems:
 
 ```Coq
 (**r Isolation.v *)
-Theorem step_preserving_inv:
-  forall st1 st2
+Theorem bpf_interpreter_preserving_inv:
+  forall fuel st1 st2 t
     (Hreg: register_inv st1)
     (Hmem: memory_inv st1)
-    (Hsem: step st1 = Some (tt, st2)),
-       register_inv st2 /\ memory_inv st2.
+    (Hver: verifier_inv st1)
+    (Hsem: bpf_interpreter fuel st1 = Some (t, st2)),
+       register_inv st2 /\ memory_inv st2 /\ verifier_inv st2.
        
-Theorem inv_avoid_undef:
-  forall st
+Theorem inv_avoid_bpf_interpreter_undef:
+  forall st f
     (Hreg: register_inv st)
-    (Hmem: memory_inv st),
-      step st <> None.       
+    (Hmem: memory_inv st)
+    (Hver: verifier_inv st),
+      bpf_interpreter f st <> None.     
 ```
-where `register_inv` is the register invariant and `memory_inv` is the memory invariant for Certirbpf.
+where `register_inv` is the register invariant, `memory_inv` is the memory invariant for Certirbpf and `verifier_inv` is the verifier invaraint.
 
 ## File struct
 - `CommonLib.v`: some common lemmas
@@ -32,38 +32,3 @@ where `register_inv` is the register invariant and `memory_inv` is the memory in
 - `MemInv.v`: the memory invariant and related lemmas
 - `IsolationLemma.v`: some lemmas used by the proof of the isolation property
 - `Isolation.v`: two target thoerems.
-
-## Proof idea
-
-The whole way to prove the theorems are do case discussion on each instruction.
-
-But there is a gap between proof idea and code generation idea: To simulate `Coq List type` correctly, we define `comm/MemType.v/MyMemRegionsType` in Coq, it use List.nth_error to access a list. This way makes the code generation easier but complex the isolation proof. Because we have a list of memory regions `Coq List type`, when we define its invariants, it natually uses native Coq List constructions `nil` and `hd::tl`, but remember we are using `nth\_error` to access the list. So it is hard to do `induction` on the list.
-
-To solve this question, we use the relation among `List.In`, `List.nth_error` and Coq List constructions!
-- `inv_memory_regions` is defined by using Coq List constructions
-- `In_inv_memory_regions` says the relation between the former and `List.In`
-- `IsolationLemma.v` uses the relation with `List.nth_error`, and complete the proof.
-```Coq
-(**r MemInv.v *)
-Fixpoint inv_memory_regions (m:mem) (mrs: list memory_region): Prop :=
-  match mrs with
-  | [] => True
-  | hd :: tl => inv_memory_region m hd /\ inv_memory_regions m tl
-  end.
-
-Lemma In_inv_memory_regions:
-  forall mr m l,
-    List.In mr l -> inv_memory_regions m l ->
-      inv_memory_region m mr.
-Proof.
-
-(**r IsolationLemma.v L773 & L805 *)
-
-  (**r we rely on the fact if Heqmr get the default memory region, check_mem_aux2P should return Vnullptr! *)
-  assert (Hdefault: check_mem_aux2P default_memory_region Readable (Vint vi) chunk = Vnullptr). {
-  ...
-  
-  (**r now we get the evidence `In mr (bpf_mrs st1)`, and reuse the lemma `In_inv_memory_regions` *)
-  apply In_inv_memory_regions with (m:=bpf_m st1) in Hin_mem_regions; [| intuition].
-
-```
